src/PermProgAuto.v
@@ -52,6 +52,8 @@ Ltac inv_exec' :=
     inv_exec'' H
   | [ H: exec _ _ _ _ _ (HashHandle2 _ _) _ _ |- _ ] =>
     inv_exec'' H
+  | [ H: exec _ _ _ _ _ (Auth _) _ _ |- _ ] =>
+    inv_exec'' H
   end.
 
 Lemma bind_sep:
